json: Clean up encoder and add decoder

src/JSON/JSON.Serializer.dfy
@@ -2,7 +2,7 @@
 ///  Serialization from JSON.AST to JSON.Grammar
 /// =============================================
 ///
-/// For the spec, see ``JSON.Spec.HighLevel.dfy``.
+/// For the spec, see ``JSON.Spec.dfy``.
 
 include "../Collections/Sequences/Seq.dfy"
 include "../BoundedInts.dfy"
@@ -11,110 +11,168 @@ include "../Math.dfy"
 include "Views.dfy"
 include "Vectors.dfy"
 include "UtfUtils.dfy"
+include "JSON.Errors.dfy"
 include "JSON.AST.dfy"
 include "JSON.Grammar.dfy"
-include "JSON.Spec.HighLevel.dfy"
-include "JSON.Spec.LowLevel.dfy"
+include "JSON.Spec.dfy"
 
 module {:options "/functionSyntax:4"} JSON.Serializer {
   import Seq
   import Math
+  import opened Wrappers
   import opened BoundedInts
   import opened Str
   import UtfUtils
 
   import AST
-  import Spec.HighLevel
+  import Spec
+  import opened Errors
   import opened Vectors
   import opened Grammar
   import opened Views.Core
 
+  type Result<+T> = SerializationResult<T>
+
   type bytes = seq<uint8>
+  type bytes32 = bs: bytes | |bs| < TWO_TO_THE_32
   type string32 = s: string | |s| < TWO_TO_THE_32
 
   function Bool(b: bool): jbool {
     View.OfBytes(if b then TRUE else FALSE)
   }
 
-  method Utf8Encode(st: Vector<uint8>, cp: uint32)
-    ensures st.Model()
-  {
+  // method Utf8Encode(st: Vector<uint8>, cp: uint32)
 
+  function Transcode16To8Escaped(str: string32, start: uint32 := 0): bytes {
+    UtfUtils.Transcode16To8(Str.EscapeQuotes(str))
+  }
+  // by method {
+  //   var len := |str| as uint32;
+  //   if len == 0 {
+  //     return [];
+  //   }
+  //   var st := new Vectors.Vector(0, len);
+  //   var c0: uint16 := 0;
+  //   var c1: uint16 := str[0] as uint16;
+  //   var idx: uint32 := 0;
+  //   while idx < len {
+  //     var c0 := c1;
+  //     var c1 := str[idx + 1] as uint16;
+  //     if c0 < 0xD800 || c0 > 0xDBFF {
+  //       Utf8Encode(st, UtfUtils.Utf16Decode1(c0));
+  //       idx := idx +1;
+  //     } else {
+  //       Utf8Encode(st, UtfUtils.Utf16Decode2(c0, c1));
+  //       idx := idx + 2;
+  //     }
+  //   }
+  // }
+
+  function CheckLength<T>(s: seq<T>, err: SerializationError): Outcome<SerializationError> {
+    Need(|s| < TWO_TO_THE_32, err)
   }
 
-  function Transcode16To8Escaped(str: string32, start: uint32 := 0): seq<uint8> {
-    UtfUtils.Transcode16To8(HighLevel.Escape(str))
-  } by method {
-    var len := |str| as uint32;
-    if len == 0 {
-      return [];
-    }
-    var st := new Vectors.Vector(0, len);
-    var c0: uint16 := 0;
-    var c1: uint16 := str[0] as uint16;
-    var idx: uint32 := 0;
-    while idx < len {
-      var c0 := c1;
-      var c1 := str[idx + 1] as uint16;
-      if c0 < 0xD800 || c0 > 0xDBFF {
-        Utf8Encode(st, UtfUtils.Utf16Decode1(c0));
-        idx := idx +1;
-      } else {
-        Utf8Encode(st, UtfUtils.Utf16Decode2(c0, c1));
-        idx := idx + 2;
-      }
-    }
-  }
-
-
-
-
-
-  function String(str: string): jstring {
-    Transcode16To8Escaped(str)
+  function String(str: string): Result<jstring> {
+    :- CheckLength(str, StringTooLong(str));
+    var bs := Transcode16To8Escaped(str);
+    :- CheckLength(bs, StringTooLong(str));
+    Success(View.OfBytes(bs))
   }
 
   function Sign(n: int): jminus {
     View.OfBytes(if n < 0 then ['-' as byte] else [])
   }
 
-  function Number(dec: AST.Decimal): jnumber {
+  module ByteStrConversion refines Str.ParametricConversion {
+    import opened BoundedInts
+    type Char = uint8
+  }
+
+  const DIGITS := [
+    '0' as uint8, '1' as uint8, '2' as uint8, '3' as uint8,
+    '4' as uint8, '5' as uint8, '6' as uint8, '7' as uint8,
+    '8' as uint8, '9' as uint8
+  ]
+
+  const MINUS := '-' as uint8
+
+  function Int'(n: int) : (str: bytes)
+    ensures forall c | c in str :: c in DIGITS || c == MINUS
+  {
+    ByteStrConversion.OfInt_any(n, DIGITS, MINUS)
+  }
+
+  function Int(n: int) : Result<View> {
+    var bs := Int'(n);
+    :- CheckLength(bs, IntTooLarge(n));
+    Success(View.OfBytes(bs))
+  }
+
+  function Number(dec: AST.Decimal): Result<jnumber> {
     var minus: jminus := Sign(dec.n);
-    var num: jnum := View.OfBytes(Str.OfInt(Math.Abs(dec.n))); // FIXME
+    var num: jnum :- Int(Math.Abs(dec.n));
     var frac: Maybe<jexp> := Empty();
-    var exp: jexp :=
+    var exp: jexp :-
       var e: je := View.OfBytes(['e' as byte]);
       var sign: jsign := Sign(dec.e10);
-      var num: jnum := View.OfBytes(Str.OfInt(Math.Abs(dec.e10)));
-      JExp(e, sign, num);
-    JNumber(minus, num, Empty, NonEmpty(exp))
+      var num: jnum :- Int(Math.Abs(dec.e10));
+      Success(JExp(e, sign, num));
+    Success(JNumber(minus, num, Empty, NonEmpty(exp)))
   }
 
-  function KV(kv: AST.KV): Suffixed<jkv, jcomma> {
-    String(kv.k) + Bytes(", ") + Value(kv.v)
-  }
-
-  function MkStructural(v: View): Structural<View> {
+  function MkStructural<T>(v: T): Structural<T> {
     Structural(EMPTY, v, EMPTY)
   }
 
-  function Object(obj: seq<AST.KV>): jobject {
-    Bracketed(MkStructural(LBRACE), [], MkStructural(RBRACE))
-    // Bytes("{") + Join(Bytes(","), Seq.Map(kv requires kv in obj => KV(kv), obj)) + Bytes("}")
+  const COLON: Structural<jcolon> :=
+    MkStructural(Grammar.COLON)
+
+  function KV(kv: (string, AST.JSON)): Result<jkv> {
+    var k :- String(kv.0);
+    var v :- Value(kv.1);
+    Success(Grammar.KV(k, COLON, v))
   }
 
-  function Array(arr: seq<AST.Value>): jarray {
-    Bracketed(MkStructural(LBRACKET), [], MkStructural(RBRACKET))
-    // Bytes("[") + Join(Bytes(","), Seq.Map(v requires v in arr => Value(v), arr)) + Bytes("]")
+  function MkSuffixedSequence<D, S>(ds: seq<D>, suffix: Structural<S>)
+    : SuffixedSequence<D, S>
+  {
+    match |ds|
+      case 0 => []
+      case 1 => [Suffixed(ds[0], Empty)]
+      case _ => [Suffixed(ds[0], NonEmpty(suffix))]
+        + MkSuffixedSequence(ds[1..], suffix)
   }
 
-  function Value(js: AST.Value): Value {
+  const COMMA: Structural<jcomma> :=
+    MkStructural(Grammar.COMMA)
+
+  function Object(obj: seq<(string, AST.JSON)>): Result<jobject> {
+    var items :- Seq.MapWithResult(v requires v in obj => KV(v), obj);
+    Success(Bracketed(MkStructural(LBRACE),
+                      MkSuffixedSequence(items, COMMA),
+                      MkStructural(RBRACE)))
+  }
+
+
+  function Array(arr: seq<AST.JSON>): Result<jarray> {
+    var items :- Seq.MapWithResult(v requires v in arr => Value(v), arr);
+    Success(Bracketed(MkStructural(LBRACKET),
+                      MkSuffixedSequence(items, COMMA),
+                      MkStructural(RBRACKET)))
+  }
+
+  function Value(js: AST.JSON): Result<Grammar.Value> {
     match js
-      case Null => Grammar.Null(View.OfBytes(NULL))
-      case Bool(b) => Grammar.Bool(Bool(b))
-      case String(str) => Grammar.String(String(str))
-      case Number(dec) => Grammar.Number(Number(dec))
-      case Object(obj) => Grammar.Object(Object(obj))
-      case Array(arr) => Grammar.Array(Array(arr))
+      case Null => Success(Grammar.Null(View.OfBytes(NULL)))
+      case Bool(b) => Success(Grammar.Bool(Bool(b)))
+      case String(str) => var s :- String(str); Success(Grammar.String(s))
+      case Number(dec) => var n :- Number(dec); Success(Grammar.Number(n))
+      case Object(obj) => var o :- Object(obj); Success(Grammar.Object(o))
+      case Array(arr) => var a :- Array(arr); Success(Grammar.Array(a))
+  }
+
+  function JSON(js: AST.JSON): Result<Grammar.JSON> {
+    var val :- Value(js);
+    Success(MkStructural(val))
   }
 }
