src/JSON/JSON.Spec.dfy
@@ -11,7 +11,7 @@ include "JSON.AST.dfy"
 include "UtfUtils.dfy"
 include "Str.dfy"
 
-module {:options "/functionSyntax:4"} JSON.Spec.HighLevel {
+module {:options "/functionSyntax:4"} JSON.Spec {
   import opened BoundedInts
 
   import opened Str
@@ -20,23 +20,16 @@ module {:options "/functionSyntax:4"} JSON.Spec.HighLevel {
 
   type bytes = seq<uint8>
 
-  function Escape(str: string): string {
-    if str == [] then []
-    else
-      (if str[0] == '\"' || str[0] == '\\' then ['\\', str[0]] else [str[0]])
-      + Escape(str[1..])
-  }
-
   function String(str: string): bytes {
-    Str.ToBytes("'") + Transcode16To8(Escape(str)) + Str.ToBytes("'")
+    Str.ToBytes("'") + Transcode16To8(Str.EscapeQuotes(str)) + Str.ToBytes("'")
   }
 
   function Number(dec: Decimal): bytes {
     Transcode16To8(Str.OfInt(dec.n)) + Str.ToBytes("e") + Transcode16To8(Str.OfInt(dec.e10))
   }
 
-  function KV(kv: KV): bytes {
-    String(kv.k) + Str.ToBytes(", ") + Value(kv.v)
+  function KV(kv: (string, JSON)): bytes {
+    String(kv.0) + Str.ToBytes(", ") + JSON(kv.1)
   }
 
   function Join(sep: bytes, items: seq<bytes>): bytes {
@@ -45,25 +38,25 @@ module {:options "/functionSyntax:4"} JSON.Spec.HighLevel {
     else items[0] + sep + Join(sep, items[1..])
   }
 
-  function Object(obj: seq<KV>): bytes {
+  function Object(obj: seq<(string, JSON)>): bytes {
     Str.ToBytes("{") +
     Join(Str.ToBytes(","), seq(|obj|, i requires 0 <= i < |obj| => KV(obj[i]))) +
     Str.ToBytes("}")
   }
 
-  function Array(arr: seq<Value>): bytes {
+  function Array(arr: seq<JSON>): bytes {
     Str.ToBytes("[") +
-    Join(Str.ToBytes(","), seq(|arr|, i requires 0 <= i < |arr| => Value(arr[i]))) +
+    Join(Str.ToBytes(","), seq(|arr|, i requires 0 <= i < |arr| => JSON(arr[i]))) +
     Str.ToBytes("]")
   }
 
-  function Value(js: Value): seq<byte> {
+  function JSON(js: JSON): bytes {
     match js
       case Null => Str.ToBytes("null")
-      case Bool(b: bool) => if b then Str.ToBytes("true") else Str.ToBytes("false")
-      case String(str: string) => String(str)
-      case Number(dec: Decimal) => Number(dec)
-      case Object(obj: seq<KV>) => Object(obj)
-      case Array(arr: seq<Value>) => Array(arr)
+      case Bool(b) => if b then Str.ToBytes("true") else Str.ToBytes("false")
+      case String(str) => String(str)
+      case Number(dec) => Number(dec)
+      case Object(obj) => Object(obj)
+      case Array(arr) => Array(arr)
   }
 }
