src/JSON/JSON.API.dfy
@@ -1,0 +1,53 @@
+include "JSON.Errors.dfy"
+include "JSON.Grammar.dfy"
+include "JSON.Spec.dfy"
+include "JSON.Serializer.dfy"
+include "JSON.ZeroCopy.Serializer.dfy"
+
+module {:options "/functionSyntax:4"} JSON.API {
+  import opened BoundedInts
+  import opened Wrappers
+  import Vs = Views.Core
+
+  import opened Errors
+  import opened AST
+  import Spec
+  import S = Serializer
+  import ZS = ZeroCopy.Serializer
+  // import Deserializer
+
+  function {:opaque} Serialize(js: JSON) : (bs: SerializationResult<seq<byte>>)
+    // TODO: Carry proofs all the way
+    // ensures bs.Success? ==> bs.value == Spec.JSON(js)
+  {
+    var js :- S.JSON(js);
+    Success(ZS.Text(js).Bytes())
+  }
+
+  method SerializeAlloc(js: JSON) returns (bs: SerializationResult<array<byte>>)
+    // TODO: Carry proofs all the way
+    // ensures bs.Success? ==> fresh(bs.value)
+    // ensures bs.Success? ==> bs.value[..] == Spec.JSON(js)
+  {
+    var js :- S.JSON(js);
+    bs := ZS.Serialize(js);
+  }
+
+  method SerializeBlit(js: JSON, bs: array<byte>) returns (len: SerializationResult<uint32>)
+    modifies bs
+    // TODO: Carry proofs all the way
+    // ensures len.Success? ==> len.value as int <= bs.Length
+    // ensures len.Success? ==> bs[..len.value] == Spec.JSON(js)
+    // ensures len.Success? ==> bs[len.value..] == old(bs[len.value..])
+    // ensures len.Failure? ==> unchanged(bs)
+  {
+    var js :- S.JSON(js);
+    len := ZS.SerializeTo(js, bs);
+  }
+
+  // function {:opaque} Deserialize(bs: seq<byte>) : (js: Result<JSON, Deserializer.Error>)
+  //   ensures js.Success? ==> bs == Spec.JSON(js.value)
+  // {
+  //   Deserializer.API.OfBytes(bs)
+  // }
+}
