src/JSON/JSON.ZeroCopy.Serializer.dfy
@@ -1,3 +1,4 @@
+include "JSON.Errors.dfy"
 include "JSON.LowLevel.Spec.dfy"
 include "JSON.LowLevel.SpecProperties.dfy"
 include "Views.Writers.dfy"
@@ -6,15 +7,14 @@ module {:options "/functionSyntax:4"} JSON.ZeroCopy.Serializer {
   import opened BoundedInts
   import opened Wrappers
 
-  import Spec
-  import SpecProperties
+  import opened Errors
+  import LowLevel.Spec
+  import LowLevel.SpecProperties
   import opened Grammar
   import opened Views.Writers
   import opened Vs = Views.Core // DISCUSS: Module naming convention?
 
-  datatype Error = OutOfMemory
-
-  method Serialize(js: JSON) returns (rbs: Result<array<byte>, Error>)
+  method Serialize(js: JSON) returns (rbs: SerializationResult<array<byte>>)
     ensures rbs.Success? ==> fresh(rbs.value)
     ensures rbs.Success? ==> rbs.value[..] == Spec.JSON(js)
   {
@@ -24,7 +24,7 @@ module {:options "/functionSyntax:4"} JSON.ZeroCopy.Serializer {
     return Success(bs);
   }
 
-  method SerializeTo(js: JSON, bs: array<byte>) returns (len: Result<uint32, Error>)
+  method SerializeTo(js: JSON, bs: array<byte>) returns (len: SerializationResult<uint32>)
     modifies bs
     ensures len.Success? ==> len.value as int <= bs.Length
     ensures len.Success? ==> bs[..len.value] == Spec.JSON(js)
