src/JSON/UtfUtils.dfy
@@ -4,7 +4,7 @@ module {:options "/functionSyntax:4"} UtfUtils {
   import opened BoundedInts
 
   function Utf16Decode1(c: uint16): uint32
-    requires c < 0xD800 || c > 0xDBFF
+    requires c < 0xD800 || 0xDBFF < c
   {
     c as uint32
   }
@@ -13,8 +13,8 @@ module {:options "/functionSyntax:4"} UtfUtils {
     requires 0xD800 <= c0 as int <= 0xDBFF
   {
     (0x10000
-      | (((c0 as bv32) & 0x03FF) << 10)
-      |  ((c1 as bv32) & 0x03FF))
+     + ((((c0 as bv32) & 0x03FF) << 10)
+       | ((c1 as bv32) & 0x03FF)))
     as uint32
   }
 
@@ -24,12 +24,12 @@ module {:options "/functionSyntax:4"} UtfUtils {
     ensures r.1 in {1, 2}
     ensures c1 == -1 ==> r.1 == 1
   {
-    if c0 < 0xD800 || c0 > 0xDBFF then
+    if c0 < 0xD800 || 0xDBFF < c0 then
       (Utf16Decode1(c0), 1)
     else if c1 >= 0 then
       (Utf16Decode2(c0, c1 as uint16), 2)
     else
-      (0xFFFD, 1)
+      (0xFFFD, 1) // Replacement character
   }
 
   function Utf16Decode(str: string): seq<uint32> {
@@ -42,24 +42,87 @@ module {:options "/functionSyntax:4"} UtfUtils {
       [cp] + Utf16Decode(str[delta..])
   }
 
-   function Utf8Encode1(cp: uint32): seq<uint8> {
+  function Utf16Encode2(cp: uint32): seq<char>
+    requires cp < 0x100000
+  {
+    var bv := cp as bv32;
+    [(0xD800 | (bv >> 10))     as char,
+     (0xDC00 | (bv  & 0x03FF)) as char]
+  }
+
+  function Utf16Encode1(cp: uint32): seq<char> {
+    if cp < 0xD800 || 0xDBFF < cp < 0x10000 then
+      [cp as char]
+    else if 0x10000 <= cp < 0x110000 then
+      Utf16Encode2(cp - 0x10000)
+    else
+      [] // Invalid: drop // TODO
+  }
+
+  function Utf16Encode(codepoints: seq<uint32>): seq<char> {
+    if codepoints == [] then []
+    else Utf16Encode1(codepoints[0]) + Utf16Encode(codepoints[1..])
+  }
+
+  function Utf8Encode1(cp: uint32): seq<uint8> {
     var bv := cp as bv32;
     if cp < 0x80 then
       [cp as uint8]
     else if cp < 0x0800 then
-      [( (bv >>  6) & 0x1F)         as uint8,
+      [(((bv >>  6) & 0x1F) | 0xC0) as uint8,
        ( (bv        & 0x3F) | 0x80) as uint8]
     else if cp < 0x10000 then
-      [( (bv >> 12) & 0x0F)         as uint8,
+      [(((bv >> 12) & 0x0F) | 0xE0) as uint8,
        (((bv >>  6) & 0x3F) | 0x80) as uint8,
-       ( (bv & 0x3F)        | 0x80) as uint8]
+       ( (bv        & 0x3F) | 0x80) as uint8]
     else if cp < 0x110000 then
-      [( (bv >> 18) & 0x07)         as uint8,
+      [(((bv >> 18) & 0x07) | 0xF0) as uint8,
        (((bv >> 12) & 0x3F) | 0x80) as uint8,
        (((bv >>  6) & 0x3F) | 0x80) as uint8,
        ( (bv        & 0x3F) | 0x80) as uint8]
     else
       [] // Invalid: drop // TODO
+  }
+
+  newtype opt_uint8 = c: int | -1 <= c as int < TWO_TO_THE_8
+
+  function Utf8DecodeChars(c0: uint8, c1: opt_uint8, c2: opt_uint8, c3: opt_uint8): (r: (uint32, uint8))
+    ensures r.1 in {1, 2, 3, 4}
+    ensures c1 == -1 ==> r.1 <= 1
+    ensures c2 == -1 ==> r.1 <= 2
+    ensures c3 == -1 ==> r.1 <= 3
+  {
+    if (c0 as bv32 & 0x80) == 0 then
+      (c0 as uint32, 1)
+    else if (c0 as bv32 & 0xE0) == 0xC0 && c1 > -1 then
+	    (( (((c0 as bv32) & 0x1F) <<  6)
+	      | ((c1 as bv32) & 0x3F       )) as uint32,
+       2)
+    else if (c0 as bv32 & 0xF0) == 0xE0 && c1 > -1 && c2 > -1 then
+      ((  (((c0 as bv32) & 0x0F) << 12)
+        | (((c1 as bv32) & 0x3F) <<  6)
+        | ( (c2 as bv32) & 0x3F       )) as uint32,
+       3)
+    else if (c0 as bv32 & 0xF8) == 0xF0 && c1 > -1 && c2 > -1 && c3 > -1 then
+      ((  (((c0 as bv32) & 0x07) << 18)
+        | (((c1 as bv32) & 0x3F) << 12)
+        | (((c2 as bv32) & 0x3F) <<  6)
+        | ( (c3 as bv32) & 0x3F       )) as uint32,
+       4)
+    else
+      (0xFFFD, 1) // Replacement character
+  }
+
+  function Utf8Decode(str: seq<uint8>): seq<uint32> {
+    if str == [] then
+      []
+    else
+      var c0 := str[0] as uint8;
+      var c1 := if |str| > 1 then str[1] as opt_uint8 else -1;
+      var c2 := if |str| > 2 then str[2] as opt_uint8 else -1;
+      var c3 := if |str| > 3 then str[3] as opt_uint8 else -1;
+      var (cp, delta) := Utf8DecodeChars(c0, c1, c2, c3);
+      [cp] + Utf8Decode(str[delta..])
   }
 
   function Utf8Encode(codepoints: seq<uint32>): seq<uint8> {
@@ -69,5 +132,9 @@ module {:options "/functionSyntax:4"} UtfUtils {
 
   function Transcode16To8(s: string): seq<uint8> {
     Utf8Encode(Utf16Decode(s))
+  }
+
+  function Transcode8To16(s: seq<uint8>): string {
+    Utf16Encode(Utf8Decode(s))
   }
 }
